src/g_simplex.mlg.d
@@ -1,0 +1,4 @@
+src/g_simplex.cmo : \
+    src/simplex_main.cmo
+src/g_simplex.cmx : \
+    src/simplex_main.cmx
