Lib/Simplex.v
@@ -1,0 +1,23 @@
+Require Import Imports.
+Require Import PolySimp.
+Require Import Psatz.
+
+Declare ML Module "simplex_plugin.plugin".
+
+Ltac simplex :=
+  call_simplex_plugin;
+  match goal with
+  | c := _ |- _ => apply checker_sound with (c := c)
+  end;
+  reflexivity.
+
+Lemma test_simplex : forall env,
+  eval_form env [
+    Add (Add (Mult (Const (-2)) (Var 1)) (Mult (Const (-3)) (Var 2))) (Const (-1));
+    Add (Add (Mult (Const 3) (Var 1)) (Neg (Var 3))) (Const 1);
+    Add (Mult (Const 9) (Var 2)) (Mult (Const 2) (Var 3))
+  ].
+Proof.
+  intros H1.
+  simplex.
+Qed.
