fake_simplex.sh
@@ -1,0 +1,3 @@
+#!/bin/bash
+echo "dummy_cert" > $2
+exit 0
